dafny/Blood.dfy
@@ -24,6 +24,7 @@ class Blood {
   requires v > 0 && u > 0;
   requires l != "" && dn != "" && de != ""
   ensures Valid();
+  modifies this;
   {
     blood_id := id;
     blood_type := b;
@@ -34,5 +35,202 @@ class Blood {
     donor_name := dn;
     donor_email := de;
     ordered := o;
+  }
+
+  method OrderBlood()
+  requires Valid();
+  ensures Valid();
+  requires ordered == false;
+  ensures ordered == true;
+  modifies this;
+  {
+    ordered := true;
+  }
+}
+
+
+predicate isRequestable(s: seq<Blood>, cd: int)
+requires forall j :: 0 <= j < |s| ==> s[j] != null && s[j].Valid();
+reads s;
+reads set x | x in s[..];
+{
+  forall j :: 0 <= j < |s| ==> !s[j].ordered &&
+    s[j].suitablity && cd <= s[j].use_by_date
+}
+
+
+predicate isDisposable(s: seq<Blood>, cd: int)
+requires forall j :: 0 <= j < |s| ==> s[j] != null && s[j].Valid();
+reads s;
+reads set x | x in s[..];
+{
+  forall j :: 0 <= j < |s| ==> !s[j].ordered &&
+    (!s[j].suitablity || cd > s[j].use_by_date)
+}
+
+
+predicate isOrdered(s: seq<Blood>)
+requires forall j :: 0 <= j < |s| ==> s[j] != null && s[j].Valid();
+reads s;
+reads set x | x in s[..];
+{
+  forall j :: 0 <= j < |s| ==> s[j].ordered
+}
+
+
+method GetRequestableBlood(s1: seq<Blood>, cd: int) returns (s2: seq<Blood>)
+requires forall j :: 0 <= j < |s1| ==> s1[j] != null && s1[j].Valid();
+ensures forall j :: 0 <= j < |s2| ==> s2[j] != null && s2[j].Valid();
+ensures 0 <= |s2| <= |s1|;
+ensures isRequestable(s2, cd);
+{
+  s2 := [];
+  var i := 0;
+  
+  while i < |s1|
+  invariant 0 <= |s2| <= i <= |s1|;
+  invariant forall j :: 0 <= j < |s1| ==> s1[j] != null && s1[j].Valid();
+  invariant forall j :: 0 <= j < |s2| ==> s2[j] != null && s2[j].Valid();
+  invariant forall j :: 0 <= j < |s2| ==> !s2[j].ordered &&
+    s2[j].suitablity && cd <= s2[j].use_by_date;
+  decreases |s1| - i;
+  {
+    if !s1[i].ordered && s1[i].suitablity 
+      && cd <= s1[i].use_by_date {
+      var s3 := [s1[i]];
+      s2 := s2 + s3;
+    }
+
+    i := i + 1;
+  }
+}
+
+
+method GetDisposableBlood(s1: seq<Blood>, cd: int) returns (s2: seq<Blood>)
+requires forall j :: 0 <= j < |s1| ==> s1[j] != null && s1[j].Valid();
+ensures forall j :: 0 <= j < |s2| ==> s2[j] != null && s2[j].Valid();
+ensures 0 <= |s2| <= |s1|;
+ensures isDisposable(s2, cd);
+{
+  s2 := [];
+  var i := 0;
+  
+  while i < |s1|
+  invariant 0 <= |s2| <= i <= |s1|;
+  invariant forall j :: 0 <= j < |s1| ==> s1[j] != null && s1[j].Valid();
+  invariant forall j :: 0 <= j < |s2| ==> s2[j] != null && s2[j].Valid();
+  invariant forall j :: 0 <= j < |s2| ==> !s2[j].ordered &&
+    (!s2[j].suitablity || cd > s2[j].use_by_date);
+  decreases |s1| - i;
+  {
+    if !s1[i].ordered && (!s1[i].suitablity 
+      || cd > s1[i].use_by_date) {
+      var s3 := [s1[i]];
+      s2 := s2 + s3;
+    }
+
+    i := i + 1;
+  }
+}
+
+
+method GetOrderedBlood(s1: seq<Blood>) returns (s2: seq<Blood>)
+requires forall j :: 0 <= j < |s1| ==> s1[j] != null && s1[j].Valid();
+ensures forall j :: 0 <= j < |s2| ==> s2[j] != null && s2[j].Valid();
+ensures 0 <= |s2| <= |s1|;
+ensures isOrdered(s2);
+{
+  s2 := [];
+  var i := 0;
+  
+  while i < |s1|
+  invariant 0 <= |s2| <= i <= |s1|;
+  invariant forall j :: 0 <= j < |s1| ==> s1[j] != null && s1[j].Valid();
+  invariant forall j :: 0 <= j < |s2| ==> s2[j] != null && s2[j].Valid();
+  invariant forall j :: 0 <= j < |s2| ==> s2[j].ordered;
+  decreases |s1| - i;
+  {
+    if s1[i].ordered {
+      var s3 := [s1[i]];
+      s2 := s2 + s3;
+    }
+
+    i := i + 1;
+  }
+}
+
+
+method Main() 
+{
+  var b1 := new Blood(1, AP, 3, true, 100, "UNSW", "John Doe", "Donor01@gmail.com", false);
+  var b2 := new Blood(2, AN, 4, true, 90, "UNSW", "Steve Doe", "Donor02@gmail.com", true);
+  var b3 := new Blood(3, BN, 8, true, 70, "UNSW", "Kate Doe", "Donor03@gmail.com", false);
+  var b4 := new Blood(4, AP, 8, false, 60, "UNSW", "Kale Doe", "Donor04@gmail.com", true);
+  var b5 := new Blood(5, OP, 4, true, 70, "UNSW", "Peter Doe", "Donor05@gmail.com", false);
+  var b6 := new Blood(6, AP, 10, true, 40, "UNSW", "Parker Doe", "Donor06@gmail.com", false);
+
+  assert b1 != null && b1.Valid();
+  assert b2 != null && b2.Valid();
+  assert b3 != null && b3.Valid();
+  assert b4 != null && b4.Valid();
+  assert b5 != null && b5.Valid();
+  assert b6 != null && b6.Valid();
+
+  var s1: seq<Blood> := [b1, b2, b3, b4, b5, b6];
+
+  assert s1[0] == b1 && s1[0] != null && s1[0].Valid();
+  assert s1[1] == b2 && s1[1] != null && s1[1].Valid();
+  assert s1[2] == b3 && s1[2] != null && s1[2].Valid();
+  assert s1[3] == b4 && s1[3] != null && s1[3].Valid();
+  assert s1[4] == b5 && s1[4] != null && s1[4].Valid();
+  assert s1[5] == b6 && s1[5] != null && s1[5].Valid();
+  assert forall j :: 0 <= j < |s1| ==> s1[j] != null && s1[j].Valid();
+
+  var s2 := GetRequestableBlood(s1, 50);
+  assert isRequestable(s2, 50);
+
+  var i := 0;
+  print "Requestable Blood", "\n";
+
+  while i < |s2|
+  invariant 0 <= i <= |s2|
+  invariant forall j :: 0 <= j < |s2| ==> s2[j] != null && s2[j].Valid();
+  decreases |s2| - i;
+  {
+    print s2[i].blood_id, " suitablity: ", s2[i].suitablity, " use_by_date: ", 
+      s2[i].use_by_date, " ordered status: ", s2[i].ordered, "\n";
+    i := i + 1;
+  }
+
+  s2 := GetDisposableBlood(s1, 50);
+  assert isDisposable(s2, 50);
+
+  i := 0;
+  print "Disposable Blood", "\n";
+
+  while i < |s2|
+  invariant 0 <= i <= |s2|
+  invariant forall j :: 0 <= j < |s2| ==> s2[j] != null && s2[j].Valid();
+  decreases |s2| - i;
+  {
+    print s2[i].blood_id, " suitablity: ", s2[i].suitablity, " use_by_date: ", 
+      s2[i].use_by_date, " ordered status: ", s2[i].ordered, "\n";
+    i := i + 1;
+  }
+
+  s2 := GetOrderedBlood(s1);
+  assert isOrdered(s2);
+
+  i := 0;
+  print "Ordered Blood", "\n";
+
+  while i < |s2|
+  invariant 0 <= i <= |s2|
+  invariant forall j :: 0 <= j < |s2| ==> s2[j] != null && s2[j].Valid();
+  decreases |s2| - i;
+  {
+    print s2[i].blood_id, " suitablity: ", s2[i].suitablity, " use_by_date: ", 
+      s2[i].use_by_date, " ordered status: ", s2[i].ordered, "\n";
+    i := i + 1;
   }
 }
